\documentclass[a4paper]{article}

%% Language and font encodings
\usepackage[english]{babel}
\usepackage[utf8x]{inputenc}
\usepackage[T1]{fontenc}

%% Sets page size and margins
\usepackage[a4paper,top=3cm,bottom=2cm,left=3cm,right=3cm,marginparwidth=1.75cm]{geometry}

%% Useful packages
\usepackage{amsmath}
\usepackage{amsfonts}
\usepackage{graphicx}
\usepackage[colorinlistoftodos]{todonotes}
\usepackage[colorlinks=true, allcolors=blue]{hyperref}

\title{Judson's Abstract Algebra: Chapter 3}
\date{}

\begin{document}
\maketitle

\section*{1}

Suppose $3x \equiv 2 \mod 7$. Then $x \in \{z: z = 3 + 7n, n \in \mathbb{Z}\}$.

\vspace{\baselineskip}

Suppose $5x + 1 \equiv 13 \mod 23$. Then $x \in \{z: z = 7 + 23n, n \in \mathbb{Z}\}$.

\vspace{\baselineskip}

Suppose $5x + 1 \equiv 13 \mod 26$. Then $x \in \{z: z = 18 + 26n, n \in \mathbb{Z}\}$.

\vspace{\baselineskip}

Suppose $9x \equiv 3 \mod 5$. Then $x \in \{z: z = 2 + 5n, n \in \mathbb{Z}\}$.

\vspace{\baselineskip}

Suppose $5x \equiv 1 \mod 6$. Then $x \in \{z: z = 5 + 6n, n \in \mathbb{Z}\}$.

\vspace{\baselineskip}

Suppose $3x \equiv 1 \mod 6$. There are no solutions.


\section*{6}

Give a multiplication table for the group $U(12)$.

\vspace{\baselineskip}

Note that $U(12) = \{ 1, 5, 7, 11 \}.$

$$
\begin{tabular}{ l | l l l l l }
  * & 1 & 5 & 7 & 11 \\
  \hline      
  1 & 1 & 5 & 7 & 11 \\
  5 & 5 & 1 & 11 & 7 \\
  7 & 7 & 11 & 1 & 5 \\
  11 & 11 & 7 & 5 & 1 \\
\end{tabular}
$$



\section*{7}

Let $S = \mathbb{R} \setminus \{ -1 \}$ and define a binary operation on $S$ by $a * b = a + b + ab$. Prove that $(S, *)$ is an abelian group.

\vspace{\baselineskip}

Let $a, b, c \in S$. The identity is 0 since $a * 0 = a + 0 + 0a = a$. The inverse of $a$ is given by 

$$ a^{-1} = \frac{-a}{1+a}$$

since

\begin{align*}
a * a^{-1} &= a * \frac{-a}{1+a} \\
&= a + \frac{-a}{1+a} + \frac{-a^2}{1+a} \\
&= \frac{a + a^2}{1+a} - \frac{a + a^2}{1+a} \\
&= 0
\end{align*}

and $a \neq -1$.

Consider

\begin{align*}
(a * b) * c &= (a + b + ab) * c \\
&= a + b + ab + c + c (a + b + ab) \\
&= a + b + c + ab + ac + bc + abc \\
&= a + (b + c + bc) + (ab + ac + abc) \\
&= a + (b * c) + a (b * c) \\
&= a * (b * c).
\end{align*}

This shows associativity.

\section*{8}

Give an example of two elements $A$ and $B$ in $GL_2(\mathbb{R})$ with $AB \neq BA$.

\vspace{\baselineskip}

Consider

$$A=
  \begin{pmatrix}
    1 & 1 \\
    0 & 1
  \end{pmatrix}
  B=
  \begin{pmatrix}
    1 & 0 \\
    1 & 1
  \end{pmatrix}.
$$

Notice

$$AB =   
  \begin{pmatrix}
    2 & 1 \\
    1 & 1
  \end{pmatrix}
$$

while 

$$BA = 
  \begin{pmatrix}
    1 & 1 \\
    1 & 2
  \end{pmatrix}
$$

\section*{9}

Prove that the product of two matrices in $SL_2(\mathbb{R})$ has determinant one.

\vspace{\baselineskip}

Let $A,B \in SL_2(\mathbb{R})$. This follows from the basic property of determinants

$$\det (AB) = \det(A) \det(B) = 1 \cdot 1 = 1.$$

\section*{10}

Prove that the set of matrices of the form
$$
  \begin{pmatrix}
    1 & x & y \\
    0 & 1 & z \\
    0 & 0 & 1
  \end{pmatrix}
$$

is a group under matrix multiplication. This group, known as the \textit{Heisenburg group}, is important in quantum physics. Matrix multiplication in the Heisenberg group is defined by

$$
  \begin{pmatrix}
    1 & x & y \\
    0 & 1 & z \\
    0 & 0 & 1
  \end{pmatrix}
  \begin{pmatrix}
    1 & x' & y' \\
    0 & 1 & z' \\
    0 & 0 & 1
  \end{pmatrix}
=
  \begin{pmatrix}
    1 & x + x' & y + y'+ xz' \\
    0 & 1 & z + z' \\
    0 & 0 & 1
  \end{pmatrix}
$$

The proof that this set of matrices forms a group is straightforward. Associativity follows from the associativity of matrix multiplication. The identity element is the usual identity matrix. Each matrix in the set is upper triangular and has an inverse (if this is not obvious, then the matrices can be easily put in reduced row echelon form).


\section*{11}

Prove that $\det(AB) = det(A)det(B)$ in $GL_2(\mathbb{R})$ Use this result to show that the binary operation in the group $GL_2(\mathbb{R})$ is closed; that is, if $A$ and $B$ are in $GL_2(\mathbb{R})$, then $AB \in GL_2(\mathbb{R})$.

\vspace{\baselineskip}

We already used this basic property of determinants in problem 9. We will prove it for $2 \times 2$ matrices here. Recall the definition of the determinant for a $2 \times 2$ matrix 
$$A = 
  \begin{pmatrix}
    a & b \\
    c & d \\
  \end{pmatrix}
$$
  
is given by $\det(A) = ad - bc$.

\vspace{\baselineskip}

Let $A,B$ be $2 \times 2$ matrices where  

$$A = 
  \begin{pmatrix}
    a & b \\
    c & d \\
  \end{pmatrix}
  B = 
  \begin{pmatrix}
    a' & b' \\
    c' & d' \\
  \end{pmatrix}
$$

and 

$$AB = 
  \begin{pmatrix}
    aa' + bc' & ab' + bd'\\
    a'c + c'd & b'c + dd' \\
  \end{pmatrix}.
$$

Notice that 

\begin{align*}
\det(AB) &= (aa' + bc')(b'c + dd') - (ab' + bd')(a'c + c'd) \\
&= aa'b'c + aa'dd' + bc'b'c + bc'dd' - ab'a'c - ab'c'd - bd'a'c - bd'c'd \\
&= (ad - bc) (a'd' - b'c') \\
&= \det(A) \det(B)
\end{align*}

\vspace{\baselineskip}

Let $C,D \in GL_2(\mathbb{R})$. Then $\det(C) \neq 0$ and $\det(D) \neq 0$. By the property proved above $\det{CD} = \det{C}\det{D}$. Since $\det{C} \neq 0$ and $\det{D} \neq 0$ we know that $\det{CD} \neq{0}$ hence $CD \in GL_2(\mathbb{R})$ and $GL_2(\mathbb{R})$ is closed.


\section*{12}

Let $\mathbb{Z}_2^n = \{ (a_1, a_2, ..., a_n) : a_i \in \mathbb{Z}_2 \}$ Define a binary operation on $\mathbb{Z}_2^n$ by 

$$(a_1, a_2, ..., a_n) + (b_1, b_2, ..., b_n) = (a_1+b_1, a_2+b_2, ..., a_n+b_n).$$

Prove that $\mathbb{Z}_2^n$ is a group under this operation. This group is important in algebraic coding theory.

\vspace{\baselineskip}

Let $(a_1, a_2, ..., a_n), (b_1, b_2, ..., b_n), (c_1, c_2, ..., c_n) \in \mathbb{Z}_2^n$. Notice that the identity is in $\mathbb{Z}_2^n$ since

$$(a_1, a_2, ..., a_n) + (0, 0, ..., 0) =  (a_1, a_2, ..., a_n).$$

Also note that each element has an inverse

$$(a_1, a_2, ..., a_n) + (-a_1, -a_2, ..., -a_n) = (0, 0, ..., 0).$$

Associativity follows from the associativity of modular arithmetic


\begin{align*}
((a_1, a_2, ..., a_n) + (b_1, b_2, ..., b_n)) + (c_1, c_2, ..., c_n) &= (a_1+b_1, a_2+b_2, ..., a_n+b_n) + (c_1, c_2, ..., c_n) \\
&= ((a_1+b_1) + c_1, (a_2+b_2) + c_2, ..., (a_n+b_n) + c_n) \\ 
&= (a_1 + (b_1+c_1), a_2 + (b_2+c_2), ..., (a_n + (b_n+c_n)) \\
&= (a_1, a_2, ..., a_n) + ((b_1, b_2, ..., b_n) + (c_1, c_2, ..., c_n)).
\end{align*}


\section*{13}

Show that $\mathbb{R}^{*} = \mathbb{R} \setminus \{ 0 \}$ is a group under the operation of multiplication.

\vspace{\baselineskip}

Let $x \in \mathbb{R}^{*}$. Notice that, since multiplication of two non-zero real numbers is non-zero,$\mathbb{R}^{*}$ is closed. Associativity follows from the associativity of the multiplication of real numbers. The identity is 1. Notice that $x^{-1} = \frac{1}{x}$ since

$$xx^{-1} = x \frac{1}{x} = 1.$$

Hence, $\mathbb{R}^*$ is a group


\section*{14}

Given the groups $\mathbb{R}^*$ and $\mathbb{Z}$ let $G = \mathbb{R} \times \mathbb{Z}$. Define a binary operation $\circ$ on $G$ by $(a,m) \circ (b,n) = (ab, m+n)$. Show that $G$ is a group under this operation.

\vspace{\baselineskip}

This proof is straightforward since the two contributing groups are operated on independently. Associativity follows from the associativity of $\mathbb{R}^*$ and $\mathbb{Z}$. The identity is $(1,0)$. The inverse of $(x, n) \in \mathbb{R}^* \times \mathbb{Z}$ is $(1/x, -n)$.

\section*{15}

The dihedral group of six elements is the smallest non-abelian group. Here is the Cayley table

\begin{tabular}{ l | l l l l l l }
  * & e & a & b & c & d & f \\
  \hline      
  e & e & a & b & c & d & f \\
  a & a & e & d & f & b & c \\
  b & b & f & e & d & c & a \\
  c & c & d & f & e & a & b \\
  d & d & c & a & b & f & e \\
  f & f & b & c & a & e & d
\end{tabular}


\section*{16}

Give a specific example of some group $G$ and elements $g, h \in G$ where $(gh)^n \neq g^n h^n$. 

\vspace{\baselineskip}

We need to find a group that is not abelian. Consider $GL_2(\mathbb{R})$. Let 

$$A = 
  \begin{pmatrix}
    1 & 2 \\
    3 & 2
  \end{pmatrix},
  B = 
  \begin{pmatrix}
    2 & 1 \\
    2 & 3
  \end{pmatrix}.
$$

Notice that 

$$A^{-1} = 
  \begin{pmatrix}
    -1/2 & 1/2 \\
    3/4 & -1/4
  \end{pmatrix},
  B^{-1} = 
  \begin{pmatrix}
    3/4 & -1/4 \\
    -1/2 & 1/2 
  \end{pmatrix}
$$

so $A, B \in GL_2(\mathbb{R})$. Then notice that 

$$A^n B^n = \begin{pmatrix}
    102 & 101 \\
    154 & 155
  \end{pmatrix} \neq 
    \begin{pmatrix}
    106 & 105 \\
    150 & 151 
  \end{pmatrix} = (AB)^n.$$

\section*{24}

Let $a$ and $B$ be elements in a group $G$. Prove that $ab^na^{-1} = (aba^{-1})^n$ for $n \in \mathbb{Z}$.

\vspace{\baselineskip}

Consider

$$ab^na^{-1} = a b ... b  a^{-1} = a  b a^{-1} a ... a^{-1} a b a^{-1} = (aba^{-1})^n.$$


\section*{25}

Let $U(n)$ be the group of units in $\mathbb{Z}_n$. If $n > 2$, prove that there is an element $k \in U(n)$ such that $k^2 = 1$ and $k \neq 1$.

\vspace{\baselineskip}




\section*{26}

Prove that the inverse of $g1 g2 ... g_n$ is $g_n^{-1} g_{n-1}^{-1} ... g_1^{-1}$.

\vspace{\baselineskip}

Consider

\begin{align*}
(g1 g2 ... g_{n-1} g_n) (g_n^{-1} g_{n-1}^{-1} ... g_2^{-1} g_1^{-1}) &= g1 g2 ... g_{n-1} g_{n-1}^{-1} ... g_2^{-1} g_1^{-1} \\
\vdots \\
&= g_1 g_2 g_2^{-1} g_1^{-1} \\
&= g_1 g_1^{-1} \\
&= e.
\end{align*}


\section*{27}

Prove the remainder of Proposition 3.6: if $G$ is a group and $a,b \in G$, then the equation $xa = b$ has unique solutions in $G$.

\vspace{\baselineskip}

Assume that $xa = b$ has more than one solution. Call two solutions $x_1, x_2$. Note that 

\begin{align*}
x_1 a &= b \\
x_1 a a^{-1} &= b a^{-1} \\
x_1 &= b a^{-1}
\end{align*}

and 

\begin{align*}
x_2 a &= b \\
x_2 a a^{-1} &= b a^{-1} \\
x_2 &= b a^{-1}
\end{align*}

Then, since the group operation is well-defined $x_1 = x_2$, a contradiction. This proves that solutions to $xa = b$ in $G$ are unique.


\section*{28}

Prove Theorem 3.8. In a group, the usual laws of exponents hold; that is, for all $g, h \in G$,

$$g^m g^n = g^{m+n} \text{ for all } m,n \in \mathbb{Z};$$
$$(g^m)^n = g^{mn} \text{ for all } m,n \in \mathbb{Z};$$
$$(gh)^n = (h^{-1} g^{-1})^{-n} \text{ for all } n \in \mathbb{Z}$$

Furthermore, if $G$ is abelian, then $(gh)^n = g^n h^n$.

\vspace{\baselineskip}

To prove the first statement, notice that (we will index for clarity where $g_i = g$)

$$g^m g^n = g_1 g_2 ... g_m g_1 ... g_n =  g^{m+n}.$$

To prove the second statement consider 

$$(g^m)^n = g^m ... g^m.$$

From the first statement it follows that 

$$(g^m ... g^m = g^{m+...+m} = g^{mn}.$$

To prove the second statement first note that

$$gh = (h^{-1} g^{-1})^{-1}.$$

It follows from the second statement that 

$$(gh)^n = ((h^{-1} g^{-1})^{-1})^n = (h^{-1} g^{-1})^{-n}.$$

Assume $G$ is abelian. Consider 

$$(gh)^n = gh .. gh = g...g h...h = g^n h^n.$$

\section*{29}

Prove the right and left cancellation laws for a group $G$; that is , show that in the group $G$, $ba = ca$ implies $b = c$ and $ab = ac$ implies $b = c$ for elements $a,b,c \in G$.

\vspace{\baselineskip}

This is a straightforward application of the existence of inverses in a  group.

Consider

\begin{align*}
ba &= ca \\
baa^{-1} &= caa^{-1} \\
be &= ce \\ 
b &= c
\end{align*}

\begin{align*}
ab &= ac \\
a^{-1}ab &= a^{-1}ac \\
eb &= ec \\
b &= c
\end{align*}


\section*{30}

Show that if $a^2 = e$ for all elements $a$ in a group $G$, then $G$ must be abelian

\vspace{\baselineskip}

Let $a,b \in G$. Consider

$$(ab)(ab) = e = (aa)(bb)$$
$$abab = aabb$$
$$ ba = ab.$$


\section*{32}

Let $G$ be a group and suppose that $(ab)^2 = a^2b^2$ for all $a$ and $b$ in $G$. Prove that $G$ is an abelian group.

\vspace{\baselineskip}

Consider

$$(ab)^2 = a^2b^2$$

$$abab = aa bb$$

multiplying on the left by $a^{-1}$ yields

$$bab = abb$$

and multiplying on the left by $b^{-1}$ yields

$$ba = ab.$$

Hence, $G$ is an abelian group.


\section*{41}

Let $G$ be the group of $2 \times 2$ matrices under addition and 

$$ H = \left\{
  \begin{pmatrix}
    a & b \\
    c & d
  \end{pmatrix} : a + d = 0\right\}.
$$

Prove that $H$ is a subgroup of $G$.

\vspace{\baselineskip}

Note that the identity is in $H$ since $0 + 0 = 0$. Consider the sum of two matrices in H

$$\begin{pmatrix}
    a & b \\
    c & d
  \end{pmatrix}
  +
  \begin{pmatrix}
    a' & b' \\
    c' & d'
  \end{pmatrix}
  =
  \begin{pmatrix}
    a + a' & b + b' \\
    c + c' & d + d'
  \end{pmatrix}.
$$

Note that since $a + a' + d + d' = 0$ we know that the sum of the matrices is also a member of $H$. Note that the inverse of a matrix $A \in H$ is given by $-A$. Let 

$$A = 
  \begin{pmatrix}
    a & b \\
    c & d
  \end{pmatrix}.
$$

Note that since $-a + -d = 0$ that $-A \in H$. This proves that $H$ is a subgroup of $G$.


\section*{44}

Prove that the intersection of two subgroups of a group $G$ is also a subgroup of $G$

\vspace{\baselineskip}

Let $H$ and $K$ be subgroups of $G$. Note that since $H$ and $K$ are subgroups, the identity element is in both and hence the identity is in $H \cap K$. Let $x,y \in H \cap K$. Note that $xy \in H$ since $x,y \in H$ and similarly $xy \in K$ since $x,y \in K$. Therefore, $xy \in H \cap K$. Note that $x^{-1} \in H$ since $x \in H$ and $x^{-1} \in K$ since $x \in K$. Therefore, $x^{-1} \in H \cap K$. This shows that $H \cap K$ is a subgroup of $G$.



\section*{45}

Prove or disprove: if $H$ and $K$ are subgroups of a group $G$, then $H \cup K$ is a subgroup of $G$.

\vspace{\baselineskip}

Consider the following counterexample. Note that $2\mathbb{Z}$ and $3\mathbb{Z}$ are both subgroups of $\mathbb{Z}$ under addition. It is clear that $2\mathbb{Z} \cup 3\mathbb{Z}$ is not a subgroup of $\mathbb{Z}$ because it is not closed under addition. For example $2,3 \in 2\mathbb{Z} \cup 3\mathbb{Z}$ but their sum $5 \not\in 2\mathbb{Z} \cup 3\mathbb{Z}$


\section*{48}

Let $a$ and $b$ be elements of a group $G$. If $a^4b = ba$ and $a^3 = e$, prove that $ab = ba$.

\vspace{\baselineskip}

Consider

\begin{align*}
ba &= a^4b \\
&= a^3 ab \\
&= ab.
\end{align*}


\section*{49}

Note that this is a duplicate of problem 48.

Let $a$ and $b$ be elements of a group $G$. If $a^4b = ba$ and $a^3 = e$, prove that $ab = ba$.
\vspace{\baselineskip}

Consider

\begin{align*}
ba &= a^4b \\
&= a^3 ab \\
&= ab.
\end{align*}


\section*{51}

If $xy = x^{-1} y^{-1}$ for all $x$ and $y$ in $G$, prove that $G$ must be abelian.

\vspace{\baselineskip}

Note 

$$x = xe = x^{-1}e = x^{-1}.$$

Consider

$$xy = (xy)^{-1} = y^{-1} x^{-1} = yx.$$


\section*{54}

Let $H$ be a subgroup of $G$. If $g \in G$, show that $gHg^{-1} = \{ghg^{-1}: h \in H \}$ is also a subgroup of $G$.

\vspace{\baselineskip}

Let $g \in G$ and $h_1, h_2 \in H$. Notice that $e = geg^{-1}$ and hence $e \in gHg^{-1}$. Notice that $gHg^{-1}$ is closed since $gh_1g^{-1} g h_2 g^{-1} = g h_1 h_2 g^{-1}$ and $H$ is closed. Note that $g h_1 g^{-1} g h_1^{-1} g^{-1} = e$. Hence, for all $x \in H$ $x^{-1} \in H$ as well. This proves that $gHg^{-1}$ is a subgroup of $G$.





\end{document}